\documentclass{article}
\usepackage{epsfig}
% Packages requested by user
\usepackage{amsmath}

\pagestyle{empty}
\begin{document}
$\textnormal{cross}(u,v)$
\pagebreak

$w$
\pagebreak

$u$
\pagebreak

$v$
\pagebreak

$A$
\pagebreak

$A^-1$
\pagebreak

\[ A * A^-1 = I \]
\pagebreak

$I$
\pagebreak

\[ ((1.0-w)*S)+(w*T)=V \]
\pagebreak

\[ w=\textnormal{Weight} \]
\pagebreak

\[ S=\textnormal{Source value} \]
\pagebreak

\[ T=\textnormal{Target value} \]
\pagebreak

\[ V=\textnormal{Interpolated value} \]
\pagebreak

\[ R*(S_v-S_0)+T_0=T_v\]
\pagebreak

\[ S_v=\textnormal{Source value} \]
\pagebreak

\[ S_0,S_1=\textnormal{Source range} \]
\pagebreak

\[ T_v=\textnormal{Target value} \]
\pagebreak

\[ T_0,T_1=\textnormal{Target range} \]
\pagebreak

\[ R=\frac{T_1-T_0}{S_1-S_0}=\textnormal{Ratio of the target to source range} \]
\pagebreak

$ax^2+bx+c=0$
\pagebreak

$f(x)=ax^2+bx+c$
\pagebreak

$x=\frac{-b\pm\sqrt{b^2-4ac}}{2a}$
\pagebreak

$x$
\pagebreak

$a$
\pagebreak

$b$
\pagebreak

$c$
\pagebreak

$P$
\pagebreak

$(1)$
\pagebreak

$P(t)=O+tD$
\pagebreak

$O$
\pagebreak

$D$
\pagebreak

$t$
\pagebreak

$(X_0,X_1)$
\pagebreak

$P(t)\in{X_0,X_1}$
\pagebreak

$X_0=O+t_0D$
\pagebreak

$t_0=\frac{X_0-O}{D}$
\pagebreak

$X_1=O+t_1D$
\pagebreak

$t_1=\frac{X_1-O}{D}$
\pagebreak

$t_0$
\pagebreak

$t_1$
\pagebreak

$0$
\pagebreak

\[ O+tD=P \]
\pagebreak

\[ O=\textnormal{Ray origin vector} \]
\pagebreak

\[ t=\textnormal{Magnitude scalar} \]
\pagebreak

\[ D=\textnormal{Ray direction vector} \]
\pagebreak

$x^2+y^2+z^2=R^2$
\pagebreak

$y$
\pagebreak

$z$
\pagebreak

$R$
\pagebreak

$(2)$
\pagebreak

$P^2+R^2=0$
\pagebreak

$(c_0,c_1,c_2$
\pagebreak

$(3)$
\pagebreak

$(x-c_0)^2+(y-c_1)^2+(z-c_2)^2=R^2$
\pagebreak

$(4)$
\pagebreak

$(P-C)^2-R^2$
\pagebreak

$(5)$
\pagebreak

$O+tD=P$
\pagebreak

$(6)$
\pagebreak

$(O+tD-C)^2-R^2=0$
\pagebreak

$(7)$
\pagebreak

$D^2t^2+2(O-C)Dt+(O-C)^2-R^2=0$
\pagebreak

$x=t$
\pagebreak

$a=D^2$
\pagebreak

$b=2D(O-C)$
\pagebreak

$c=(O-C)^2-R^2$
\pagebreak

\[ AI=A\]
\pagebreak

\[ A=\textnormal{Any matrix} \]
\pagebreak

\[ I=\textnormal{Identity matrix} \]
\pagebreak

$M\textnormal{x}N$
\pagebreak

$1$
\pagebreak

\[ \begin{bmatrix} 1 & 0 & \cdots & & 0 \\ 0 & 1 & & & \\ \vdots & & \ddots & & \vdots \\ & & & 1 & 0 \\ 0 & & \cdots & 0 & 1 \end{bmatrix} \]
\pagebreak

$\theta$
\pagebreak

\[ \begin{bmatrix} 1 & 0 & 0 & 0 \\ 0 & cos\theta & -sin\theta & 0 \\ 0 & sin\theta & cos\theta & 0 \\ 0 & 0 & 0 & 1 \end{bmatrix} \]
\pagebreak

\[ \begin{bmatrix} cos\theta & 0 & sin\theta & 0 \\ 0 & 1 & 0 & 0 \\ -sin\theta & 0 & cos\theta & 0 \\ 0 & 0 & 0 & 1 \end{bmatrix} \]
\pagebreak

\[ \begin{bmatrix} cos\theta & -sin\theta & 0 & 0 \\ sin\theta & cos\theta & 0 & 0 \\ 0 & 0 & 1 & 0 \\ 0 & 0 & 0 & 1 \end{bmatrix} \]
\pagebreak

$S=(S_x,S_y,S_z)$
\pagebreak

\[ \begin{bmatrix} S_x & 0 & 0 & 0 \\ 0 & S_y & 0 & 0 \\ 0 & 0 & S_z & 0 \\ 0 & 0 & 0 & 1 \end{bmatrix} \]
\pagebreak

$T=(T_x,T_y,T_z)$
\pagebreak

\[ \begin{bmatrix} 1 & 0 & 0 & T_x \\ 0 & 1 & 0 & T_y \\ 0 & 0 & 1 & T_z \\ 0 & 0 & 0 & 1 \end{bmatrix} \]
\pagebreak

\end{document}
